Start work on lemma 2.10
This is the grungy bit to do with tracking rho on V(sigma V). It
remains to show that the function is injective on the image. Then we
just have to use the injection in FPCard in one direction and glue
everything together.

Terms/Generality.v
@@ -6,6 +6,7 @@ Require Import Top.Terms.VecUtils.
 Require Import Top.FinSet.FinSet.
 Require Import Top.FinSet.FinMod.
 
+
 (* First, we have to define the "more general than" relation on
    substitutions, abbreviated to smg.
  *)
@@ -61,15 +62,86 @@ End smg.
     that if two substitutions are equivalent under the [smg] relation then
     there are permutations that relabel them into each other.
 
-    The first big statement is that if you have a finite substitution, sigma,
-    then there are only finitely many variables that are not free variables in
-    the image of sigma. Why? Well, sigma leaves all but finitely many variables
-    untouched and these untouched variables will still be free in the image of
-    sigma.
-
-    We start by setting up a sigma type for the bound variables. We want to
-    show that [proj1_sig] on that sigma type is a finite projection.
-
-    TODO: Currently working on this in the BoundInImage module.
-
 *)
+Section sequiv_means_perm.
+  Variable L : lType.
+  Variables sigma sigma' : Subst L.
+  Variables rho rho' : Subst L.
+  Hypothesis sigma'H : forall v, sigma' v = comp_subst rho sigma v.
+  Hypothesis sigmaH : forall v, sigma v = comp_subst rho' sigma' v.
+
+  Lemma sigma_is_rho2_sigma v
+    : sigma v = comp_subst (comp_subst rho' rho) sigma v.
+  Proof.
+    rewrite <- comp_subst_assoc.
+    unfold comp_subst at 1, compose; simpl.
+    rewrite <- sigma'H, sigmaH; auto.
+  Qed.
+
+  Lemma rho2_fixes_im_sigma v
+    : termset_fv v (subst_im sigma) ->
+      comp_subst rho' rho v = varTerm L v.
+  Proof.
+    apply (@comp_subst_determines_fvs
+             L sigma (comp_subst rho' rho) (varTerm L)); clear v.
+    intro v; rewrite <- sigma_is_rho2_sigma, comp_subst_idl; auto.
+  Qed.
+
+  Lemma rho_im_sigma_has_height_0 v
+    : termset_fv v (subst_im sigma) -> term_height (rho v) = 0.
+  Proof.
+    intro fvH.
+    apply PeanoNat.Nat.le_0_r.
+    apply (PeanoNat.Nat.le_trans _ _ _ (@term_height_comp_subst L rho' rho v)).
+    rewrite (rho2_fixes_im_sigma v fvH); auto.
+  Qed.
+
+  Definition unpack_height_0_term (t : Term L)
+    : term_height t = 0 -> Term.V L :=
+    match t with
+    | varTerm _ v => fun _ => v
+    | funTerm f ts =>
+      fun htH =>
+        False_rect (Term.V L)
+                   (PeanoNat.Nat.neq_succ_0
+                      (vec_max_at (term_height (L:=L)) ts) htH)
+    end.
+
+  Lemma varTerm_unpack_height_0_term t H
+    : varTerm L (unpack_height_0_term t H) = t.
+  Proof.
+    destruct t; auto.
+    contradiction (PeanoNat.Nat.neq_succ_0 _ H).
+  Qed.
+
+  Definition rho_v_var_on_im_sigma
+             (v : Term.V L) (fvH : termset_fv v (subst_im sigma)) : Term.V L :=
+    unpack_height_0_term (rho v) (rho_im_sigma_has_height_0 v fvH).
+
+  Lemma rvvois_correct
+        v (fvH : termset_fv v (subst_im sigma))
+    : varTerm L (rho_v_var_on_im_sigma v fvH) = rho v.
+  Proof.
+    apply varTerm_unpack_height_0_term.
+  Qed.
+
+  Lemma rvvois_is_fv_for_sigma'
+        v (fvH : termset_fv v (subst_im sigma))
+    : termset_fv (rho_v_var_on_im_sigma v fvH) (subst_im sigma').
+  Proof.
+    destruct fvH as [ t [ imH fvH' ] ].
+    generalize (ex_intro (fun t0 => _ /\ term_fv v t0) _
+                         (conj imH fvH')); intro fvH.
+    destruct imH as [ w tH ].
+    rewrite tH in fvH'; clear t tH.
+    rewrite termset_fv_subst_im; exists w.
+    rewrite sigma'H.
+    apply (term_fv_in_subst_endo rho v
+                                 (rho_v_var_on_im_sigma v fvH)
+                                 (sigma w)
+                                 fvH').
+    rewrite <- (rvvois_correct v fvH).
+    simpl; auto.
+  Qed.
+
+End sequiv_means_perm.
